memory_ops_solvers.v
@@ -1,0 +1,116 @@
+Require Import Arith.  
+Require Import Nat.
+Require Import Bool.
+Require Import bbv.Word.
+Require Import Coq.NArith.NArith.
+Require Import List.
+Import ListNotations.
+Require Import Coq.Logic.FunctionalExtensionality.
+
+Require Import FORVES2.constants.
+Import Constants.
+
+Require Import FORVES2.program.
+Import Program.
+
+Require Import FORVES2.execution_state.
+Import ExecutionState.
+
+Require Import FORVES2.stack_operation_instructions.
+Import StackOpInstrs.
+
+Require Import FORVES2.misc.
+Import Misc.
+
+Require Import FORVES2.symbolic_state.
+Import SymbolicState.
+
+Require Import FORVES2.symbolic_state_eval.
+Import SymbolicStateEval.
+
+Require Import FORVES2.valid_symbolic_state.
+Import ValidSymbolicState.
+
+Require Import FORVES2.symbolic_state_cmp.
+Import SymbolicStateCmp.
+
+Require Import FORVES2.constraints.
+Import Constraints.
+
+Module MemoryOpsSolvers.
+
+(* ctx sv smem m ops -> smap_value *)
+Definition mload_solver_type := constraints -> sstack_val -> smemory -> smap -> stack_op_instr_map -> smap_value.
+
+Definition mload_solver_ext_type := sstack_val_cmp_ext_1_t -> mload_solver_type.
+
+Definition mload_solver_valid_res (mload_solver: mload_solver_type) :=
+  forall ctx m smem soffset smv ops,
+    is_sat ctx -> (* this is not really required *)
+    valid_smemory (get_maxidx_smap m) smem -> (* The memory is valid *)
+    valid_sstack_value (get_maxidx_smap m) soffset -> (* The offset is valid *)    
+    mload_solver ctx soffset smem m ops = smv ->
+    valid_smap_value (get_maxidx_smap m) ops smv.
+
+Definition mload_solver_correct_res (mload_solver: mload_solver_type) :=
+  forall ctx m smem soffset smv ops idx1 m1,
+    is_sat ctx ->
+    valid_smap (get_maxidx_smap m) (get_bindings_smap m) ops -> (* The smap is valid *)
+    valid_smemory (get_maxidx_smap m) smem -> (* The memory is valid *)
+    valid_sstack_value (get_maxidx_smap m) soffset -> (* The offset is valid *)    
+    mload_solver ctx soffset smem m ops = smv -> (* The value was resolved *)
+    add_to_smap m smv = (idx1, m1) ->
+    exists idx2 m2,
+      add_to_smap m (SymMLOAD soffset smem) = (idx2, m2) /\
+        forall model mem strg exts,
+          is_model ctx model = true ->
+          exists v,
+            eval_sstack_val(FreshVar idx1) model mem strg exts (get_maxidx_smap m1) (get_bindings_smap m1) ops = Some v /\
+              eval_sstack_val(FreshVar idx2) model mem strg exts (get_maxidx_smap m2) (get_bindings_smap m2) ops = Some v.
+
+Definition mload_solver_snd (mload_solver: mload_solver_type) :=
+  mload_solver_valid_res mload_solver /\ mload_solver_correct_res mload_solver.
+
+Definition mload_solver_ext_snd (mload_solver: mload_solver_ext_type) :=
+  forall sstack_val_cmp,
+    safe_sstack_val_cmp_ext_1 sstack_val_cmp ->
+    mload_solver_snd (mload_solver sstack_val_cmp).
+
+
+(* ctx u smem m ops -> smem' *)
+Definition smemory_updater_type := constraints -> memory_update sstack_val -> smemory -> smap -> stack_op_instr_map -> smemory.
+
+Definition smemory_updater_ext_type := sstack_val_cmp_ext_1_t -> smemory_updater_type.
+
+
+Definition smemory_updater_valid_res (smemory_updater: smemory_updater_type) :=
+  forall ctx m smem smem' u ops,
+    is_sat ctx -> (* this is not really required *)
+    valid_smemory (get_maxidx_smap m) smem -> (* The memory is valid *)
+    valid_smemory_update (get_maxidx_smap m) u -> (* The update is valid *)    
+    smemory_updater ctx u smem m ops = smem' ->
+    valid_smemory (get_maxidx_smap m) smem'. (* The new memory is valid *)
+
+Definition smemory_updater_correct_res (smemory_updater: smemory_updater_type) :=
+  forall ctx m smem smem' u ops,
+    is_sat ctx ->
+    valid_smap (get_maxidx_smap m) (get_bindings_smap m) ops -> (* The smap is valid *)
+    valid_smemory (get_maxidx_smap m) smem -> (* The memory is valid *)
+    valid_smemory_update (get_maxidx_smap m) u -> (* The update is valid *)    
+    smemory_updater ctx u smem m ops = smem' ->
+    forall model mem strg exts,
+      is_model ctx model = true ->
+      exists mem1 mem2,
+        eval_smemory (u::smem) (get_maxidx_smap m) (get_bindings_smap m) model mem strg exts ops = Some mem1 /\
+          eval_smemory smem' (get_maxidx_smap m) (get_bindings_smap m) model mem strg exts ops = Some mem2 /\
+          eq_memory mem1 mem2.
+
+Definition smemory_updater_snd (smemory_updater: smemory_updater_type) :=
+  smemory_updater_valid_res smemory_updater /\ smemory_updater_correct_res smemory_updater.
+
+Definition smemory_updater_ext_snd (smemory_updater: smemory_updater_ext_type) :=
+  forall sstack_val_cmp,
+    safe_sstack_val_cmp_ext_1 sstack_val_cmp ->
+    smemory_updater_snd (smemory_updater sstack_val_cmp).
+
+End MemoryOpsSolvers.
