symbolic_state_cmp.v
@@ -1,0 +1,505 @@
+Require Import Arith.
+Require Import Nat.
+Require Import Bool.
+Require Import bbv.Word.
+Require Import Coq.NArith.NArith.
+Require Import List.
+Import ListNotations.
+
+Require Import FORVES2.constants.
+Import Constants.
+
+Require Import FORVES2.program.
+Import Program.
+
+Require Import FORVES2.execution_state.
+Import ExecutionState.
+
+Require Import FORVES2.stack_operation_instructions.
+Import StackOpInstrs.
+
+Require Import FORVES2.misc.
+Import Misc.
+
+Require Import FORVES2.symbolic_state.
+Import SymbolicState.
+
+Require Import FORVES2.symbolic_state_eval.
+Import SymbolicStateEval.
+
+
+Require Import FORVES2.valid_symbolic_state.
+Import ValidSymbolicState.
+
+Require Import FORVES2.concrete_interpreter.
+Import ConcreteInterpreter.
+
+Require Import FORVES2.eval_common.
+Import EvalCommon.
+
+Require Import FORVES2.constraints.
+Import Constraints.
+
+Module SymbolicStateCmp.
+
+
+Definition symbolic_state_cmp := constraints -> sstate -> sstate -> stack_op_instr_map -> bool.
+
+
+(* Enrique: version with eval_sstate *)
+Definition symbolic_state_cmp_snd (f_cmp : symbolic_state_cmp) :=
+  forall sst1 sst2 ops ctx,
+    is_sat ctx ->
+    valid_sstate sst1 ops ->
+    valid_sstate sst2 ops ->
+    f_cmp ctx sst1 sst2 ops = true ->
+    forall mem strg exts model,
+      is_model ctx model = true ->
+      exists st',
+        eval_sstate sst1 model mem strg exts ops = Some st' /\
+          eval_sstate sst2 model mem strg exts ops = Some st'.
+
+
+(* Definition of symbolic state comparator *)
+
+(* Trivially sound comparator that always returns false *)
+Definition dummy_symbolic_state_cmp : symbolic_state_cmp :=
+  fun (ctx: constraints) =>
+  fun (sst1: sstate) =>
+  fun (sst2: sstate) =>
+  fun (ops: stack_op_instr_map) => 
+  false.
+  
+Lemma dummy_symbolic_state_cmp_snd: symbolic_state_cmp_snd dummy_symbolic_state_cmp.
+Proof.
+  unfold symbolic_state_cmp_snd.
+  intros sst1 sst2 ops instk_height Hdummy.
+  unfold dummy_symbolic_state_cmp in Hdummy.
+  discriminate.
+Qed.
+
+
+
+(* ctx sv1 sv2 maxidx1 sb1 maxid2 sb2 ops -> bool *)
+Definition sstack_val_cmp_t := constraints -> sstack_val -> sstack_val -> nat -> sbindings -> nat -> sbindings -> stack_op_instr_map -> bool.
+
+(* ctx smem1 smem2 maxidx1 sb1 maxid2 sb2 ops -> bool *)
+Definition smemory_cmp_t := constraints -> smemory -> smemory -> nat -> sbindings -> nat -> sbindings -> stack_op_instr_map -> bool.
+(* sstack_val_cmp ctx smem1 smem2 maxidx1 sb1 maxid2 sb2 ops -> bool *)
+Definition smemory_cmp_ext_t := sstack_val_cmp_t -> smemory_cmp_t.
+
+(* ctx sstrg1 sstrg2 maxidx1 sb1 maxid2 sb2 ops -> bool *)
+Definition sstorage_cmp_t := constraints -> sstorage -> sstorage -> nat -> sbindings -> nat -> sbindings -> stack_op_instr_map -> bool.
+(* sstack_val_cmp ctx sstrg1 sstrg2 maxidx1 sb1 maxid2 sb2 ops -> bool *)
+Definition sstorage_cmp_ext_t := sstack_val_cmp_t -> sstorage_cmp_t.
+
+(* ctx soffset1 ssize1 smem1 soffset2 ssize2 smem2 maxidx1 sb1 maxid2 sb2 ops -> bool *)
+Definition sha3_cmp_t := constraints -> sstack_val -> sstack_val -> smemory -> sstack_val -> sstack_val -> smemory -> nat -> sbindings -> nat -> sbindings -> stack_op_instr_map -> bool.
+(* sstack_val_cmp ctx soffset1 ssize1 smem1 soffset2 ssize2 smem2 maxidx1 sb1 maxid2 sb2 instk_height ops -> bool *)
+Definition sha3_cmp_ext_t  := sstack_val_cmp_t -> sha3_cmp_t.
+
+
+(* d ctx sv1 sv2 maxidx1 sb1 maxid2 sb2 ops -> bool *)
+Definition sstack_val_cmp_ext_1_t := nat -> sstack_val_cmp_t.
+(* smemory_cmp sstorage_cmp sha3_cmp d ctx sv1 sv2 maxidx1 sb1 maxid2 sb2 instk_height ops -> bool *)
+Definition sstack_val_cmp_ext_2_t := smemory_cmp_ext_t -> sstorage_cmp_ext_t -> sha3_cmp_ext_t -> sstack_val_cmp_ext_1_t.
+
+
+(* Comparing stack value always fail for d=0 (d is used to bound
+recursion depth, have a decreasing argument, and to make some circular
+dependencies between lemmas inductive *)
+Definition sstack_val_cmp_fail_for_d_eq_0 (sstack_value_cmp: sstack_val_cmp_ext_2_t) :=
+  forall smemory_cmp sstorage_cmp sha3_cmp ctx sv1 sv2 maxidx1 sb1 maxidx2 sb2 ops,
+   sstack_value_cmp smemory_cmp sstorage_cmp sha3_cmp 0 ctx sv1 sv2 maxidx1 sb1 maxidx2 sb2 ops = false.
+
+Definition safe_smemory_cmp (smemory_cmp: smemory_cmp_t) :=
+  forall ctx smem1 smem2 maxidx1 sb1 maxidx2 sb2 ops,
+    is_sat ctx ->
+    valid_bindings maxidx1 sb1 ops ->
+    valid_bindings maxidx2 sb2 ops ->
+    valid_smemory  maxidx1 smem1 ->
+    valid_smemory  maxidx2 smem2 ->
+    smemory_cmp ctx smem1 smem2 maxidx1 sb1 maxidx2 sb2 ops = true ->
+    forall model mem strg exts,
+      is_model ctx model = true ->
+      exists mem',
+           eval_smemory smem1 maxidx1 sb1 model mem strg exts ops = Some mem' /\
+             eval_smemory smem2 maxidx2 sb2 model mem strg exts ops = Some mem'.
+
+Definition safe_sstorage_cmp (sstorage_cmp: sstorage_cmp_t) :=
+  forall ctx sstrg1 sstrg2 maxidx1 sb1 maxidx2 sb2 ops,
+    is_sat ctx ->
+    valid_bindings maxidx1 sb1 ops ->
+    valid_bindings maxidx2 sb2 ops ->
+    valid_sstorage maxidx1 sstrg1 ->
+    valid_sstorage maxidx2 sstrg2 ->
+    sstorage_cmp ctx sstrg1 sstrg2 maxidx1 sb1 maxidx2 sb2 ops = true ->
+    forall model mem strg exts,
+      is_model ctx model = true ->
+      exists strg',
+        eval_sstorage sstrg1 maxidx1 sb1 model mem strg exts ops = Some strg' /\
+          eval_sstorage sstrg2 maxidx2 sb2 model mem strg exts ops = Some strg'.
+
+Definition safe_sha3_cmp (sha3_cmp: sha3_cmp_t) :=
+  forall ctx soffset1 ssize1 smem1 soffset2 ssize2 smem2 maxidx1 sb1 maxidx2 sb2 ops,
+    is_sat ctx ->
+    valid_sstack_value maxidx1 soffset1 ->
+    valid_sstack_value maxidx1 ssize1 ->
+    valid_sstack_value maxidx2 soffset2 ->
+    valid_sstack_value maxidx2 ssize2 ->
+    valid_bindings maxidx1 sb1 ops ->
+    valid_bindings maxidx2 sb2 ops ->
+    valid_smemory maxidx1 smem1 ->
+    valid_smemory maxidx2 smem2 ->
+    sha3_cmp ctx soffset1 ssize1 smem1 soffset2 ssize2 smem2 maxidx1 sb1 maxidx2 sb2 ops = true ->
+    forall model mem strg exts,
+      is_model ctx model = true ->
+      exists offset1 size1 mem1 offset2 size2 mem2 v,
+      eval_smemory smem1 maxidx1 sb1 model mem strg exts ops = Some mem1 /\
+      eval_smemory smem2 maxidx2 sb2 model mem strg exts ops = Some mem2 /\
+      eval_sstack_val soffset1 model mem strg exts maxidx1 sb1 ops = Some offset1 /\
+      eval_sstack_val ssize1 model mem strg exts maxidx1 sb1 ops = Some size1 /\
+      eval_sstack_val soffset2 model mem strg exts maxidx2 sb2 ops = Some offset2 /\
+      eval_sstack_val ssize2 model mem strg exts maxidx2 sb2 ops = Some size2 /\
+      (get_sha3_info_op (get_keccak256_exts exts)) (wordToNat size1) (mload' mem1 offset1 (wordToNat size1)) = v /\
+      (get_sha3_info_op (get_keccak256_exts exts)) (wordToNat size2) (mload' mem2 offset2 (wordToNat size2)) = v.
+
+Definition safe_sstack_val_cmp (f_cmp : sstack_val_cmp_t) :=
+  forall ctx sv1 sv2 maxidx1 sb1 maxidx2 sb2 ops,
+    is_sat ctx ->
+    valid_sstack_value maxidx1 sv1 ->
+    valid_sstack_value maxidx2 sv2 ->
+    valid_bindings maxidx1 sb1 ops ->
+    valid_bindings maxidx2 sb2 ops ->
+    f_cmp ctx sv1 sv2 maxidx1 sb1 maxidx2 sb2 ops = true ->
+    forall model mem strg exts,
+      is_model ctx model = true ->
+      exists v,
+        eval_sstack_val sv1 model mem strg exts maxidx1 sb1 ops = Some v /\
+          eval_sstack_val sv2 model mem strg exts maxidx2 sb2 ops = Some v.
+
+Definition safe_smemory_cmp_ext_d (smemory_cmp: smemory_cmp_ext_t) (sstack_val_cmp: sstack_val_cmp_ext_1_t) (d: nat) :=
+    forall d', d' <= d -> safe_smemory_cmp (smemory_cmp (sstack_val_cmp d')).
+
+Definition safe_sstorage_cmp_ext_d (sstorage_cmp: sstorage_cmp_ext_t) (sstack_val_cmp: sstack_val_cmp_ext_1_t) (d: nat) :=
+    forall d', d' <= d -> safe_sstorage_cmp (sstorage_cmp (sstack_val_cmp d')).
+
+Definition safe_sha3_cmp_ext_d (sha3_cmp: sha3_cmp_ext_t) (sstack_val_cmp: sstack_val_cmp_ext_1_t) (d: nat) :=
+    forall d', d' <= d -> safe_sha3_cmp (sha3_cmp (sstack_val_cmp d')).
+
+
+Definition safe_sstack_val_cmp_ext_1_d (sstack_val_cmp: sstack_val_cmp_ext_1_t) (d: nat) :=
+  forall d', d' <= d -> safe_sstack_val_cmp (sstack_val_cmp d').
+
+Definition safe_sstack_val_cmp_ext_2_d (sstack_val_cmp: sstack_val_cmp_ext_2_t) (smemory_cmp: smemory_cmp_ext_t) (sstorage_cmp: sstorage_cmp_ext_t) (sha3_cmp: sha3_cmp_ext_t)  (d: nat) :=
+    safe_sstack_val_cmp_ext_1_d (sstack_val_cmp smemory_cmp sstorage_cmp sha3_cmp) d.
+
+
+Definition safe_smemory_cmp_ext (smemory_cmp: smemory_cmp_ext_t) (sstack_val_cmp: sstack_val_cmp_ext_1_t) :=
+  forall d, safe_smemory_cmp_ext_d smemory_cmp sstack_val_cmp d.
+
+Definition safe_sstorage_cmp_ext (sstorage_cmp: sstorage_cmp_ext_t) (sstack_val_cmp: sstack_val_cmp_ext_1_t) :=
+  forall d, safe_sstorage_cmp_ext_d sstorage_cmp sstack_val_cmp d.
+
+Definition safe_sha3_cmp_ext (sha3_cmp: sha3_cmp_ext_t) (sstack_val_cmp: sstack_val_cmp_ext_1_t) :=
+  forall d, safe_sha3_cmp_ext_d sha3_cmp sstack_val_cmp d.
+
+Definition safe_sstack_val_cmp_ext_2 (sstack_val_cmp: sstack_val_cmp_ext_2_t) (smemory_cmp: smemory_cmp_ext_t) (sstorage_cmp: sstorage_cmp_ext_t) (sha3_cmp: sha3_cmp_ext_t)  :=
+  forall d, safe_sstack_val_cmp_ext_2_d sstack_val_cmp smemory_cmp sstorage_cmp sha3_cmp d.
+
+Definition safe_sstack_val_cmp_ext_1 (sstack_val_cmp: sstack_val_cmp_ext_1_t) :=
+  forall d, safe_sstack_val_cmp_ext_1_d sstack_val_cmp d.
+
+
+
+Definition safe_smemory_cmp_ext_wrt_sstack_value_cmp (smemory_cmp: smemory_cmp_ext_t) :=
+  forall (d: nat) (sstack_val_cmp: sstack_val_cmp_ext_1_t),
+    safe_sstack_val_cmp_ext_1_d sstack_val_cmp d ->
+    safe_smemory_cmp_ext_d smemory_cmp sstack_val_cmp d.
+
+Definition safe_sstorage_cmp_ext_wrt_sstack_value_cmp (sstorage_cmp: sstorage_cmp_ext_t) :=
+  forall (d: nat) (sstack_val_cmp: sstack_val_cmp_ext_1_t),
+    safe_sstack_val_cmp_ext_1_d sstack_val_cmp d ->
+    safe_sstorage_cmp_ext_d sstorage_cmp sstack_val_cmp d.
+
+Definition safe_sha3_cmp_ext_wrt_sstack_value_cmp  (sha3_cmp: sha3_cmp_ext_t) :=
+  forall (d: nat) (sstack_val_cmp: sstack_val_cmp_ext_1_t),
+    safe_sstack_val_cmp_ext_1_d sstack_val_cmp d ->
+    safe_sha3_cmp_ext_d sha3_cmp sstack_val_cmp d.
+
+Definition safe_sstack_value_cmp_wrt_others (sstack_val_cmp: sstack_val_cmp_ext_2_t) :=
+  forall (d: nat) (smemory_cmp: smemory_cmp_ext_t) (sstorage_cmp: sstorage_cmp_ext_t) (sha3_cmp: sha3_cmp_ext_t),   
+    safe_smemory_cmp_ext_d smemory_cmp (sstack_val_cmp smemory_cmp sstorage_cmp sha3_cmp) d ->
+    safe_sstorage_cmp_ext_d sstorage_cmp (sstack_val_cmp smemory_cmp sstorage_cmp sha3_cmp) d ->
+    safe_sha3_cmp_ext_d sha3_cmp (sstack_val_cmp smemory_cmp sstorage_cmp sha3_cmp) d ->
+    safe_sstack_val_cmp_ext_2_d sstack_val_cmp smemory_cmp sstorage_cmp sha3_cmp (S d).
+
+Lemma forall_dist_over_and:
+  forall (P1 P2 : nat -> Prop),
+    (forall d, P1 d /\ P2 d) <->
+              ((forall d, P1 d)/\(forall d, P2 d)).
+Proof.
+  intros.
+  split.
+  - split.
+    + intro. apply H.
+    + intro. apply H.
+  - intuition.
+Qed.
+
+Lemma safe_ext_2_implies_safe_ext_1:
+  forall d smemory_cmp sstorage_cmp sha3_cmp sstack_val_cmp,
+    safe_sstack_val_cmp_ext_2_d sstack_val_cmp smemory_cmp sstorage_cmp sha3_cmp d ->
+    safe_sstack_val_cmp_ext_1_d (sstack_val_cmp smemory_cmp sstorage_cmp sha3_cmp) d.
+Proof.
+  intros d smemory_cmp sstorage_cmp sha3_cmp sstack_val_cmp H_ext_2.
+  unfold safe_sstack_val_cmp_ext_2_d in H_ext_2.
+  unfold safe_sstack_val_cmp_ext_1_d.
+  apply H_ext_2.
+Qed.
+
+
+Lemma safe_ext_smemory_sstorage_sha3_cmp:
+  forall (smemory_cmp: smemory_cmp_ext_t) (sstorage_cmp: sstorage_cmp_ext_t) (sha3_cmp: sha3_cmp_ext_t) (sstack_val_cmp: sstack_val_cmp_ext_2_t),
+    sstack_val_cmp_fail_for_d_eq_0 sstack_val_cmp ->
+    safe_smemory_cmp_ext_wrt_sstack_value_cmp smemory_cmp ->
+    safe_sstorage_cmp_ext_wrt_sstack_value_cmp sstorage_cmp ->
+    safe_sha3_cmp_ext_wrt_sstack_value_cmp sha3_cmp ->
+    safe_sstack_value_cmp_wrt_others sstack_val_cmp ->
+    safe_smemory_cmp_ext smemory_cmp (sstack_val_cmp smemory_cmp sstorage_cmp sha3_cmp)/\
+    safe_sstorage_cmp_ext sstorage_cmp (sstack_val_cmp smemory_cmp sstorage_cmp sha3_cmp) /\
+    safe_sha3_cmp_ext sha3_cmp (sstack_val_cmp smemory_cmp sstorage_cmp sha3_cmp).
+Proof.
+  intros smemory_cmp sstorage_cmp sha3_cmp sstack_val_cmp H_d0 H_s_mem H_s_strg H_s_sha3 H_s_ssval.
+
+  unfold safe_smemory_cmp_ext.
+  unfold safe_sstorage_cmp_ext.
+  unfold safe_sha3_cmp_ext.
+  unfold safe_smemory_cmp_ext_wrt_sstack_value_cmp in H_s_mem.
+  unfold safe_sstorage_cmp_ext_wrt_sstack_value_cmp in H_s_strg.
+  unfold safe_sha3_cmp_ext_wrt_sstack_value_cmp in H_s_sha3.
+  unfold safe_sstack_value_cmp_wrt_others in H_s_ssval.
+  
+  rewrite <- forall_dist_over_and.
+  rewrite <- forall_dist_over_and.
+  
+  induction d as [|d'].
+  - split.
+    + apply H_s_mem.
+      unfold safe_sstack_val_cmp_ext_1_d.
+      intros d' H_d'_le_0.
+      apply Nat.leb_le in H_d'_le_0 as H_d'_le_0_leb.
+      unfold safe_sstack_val_cmp.
+      intros.
+      destruct d'; try discriminate.
+      unfold sstack_val_cmp_fail_for_d_eq_0 in H_d0.
+      pose proof (H_d0 smemory_cmp sstorage_cmp sha3_cmp ctx sv1 sv2 maxidx1 sb1 maxidx2 sb2 ops).
+      rewrite H6 in H4.
+      discriminate H4.
+    + split.
+      * apply H_s_strg.
+        unfold safe_sstack_val_cmp_ext_1_d.
+        intros d' H_d'_le_0.
+        apply Nat.leb_le in H_d'_le_0 as H_d'_le_0_leb.
+        unfold safe_sstack_val_cmp.
+        intros.
+        destruct d'; try discriminate.
+        unfold sstack_val_cmp_fail_for_d_eq_0 in H_d0.
+        pose proof (H_d0 smemory_cmp sstorage_cmp sha3_cmp ctx sv1 sv2 maxidx1 sb1 maxidx2 sb2 ops).
+        rewrite H6 in H4.
+        discriminate.
+      * apply H_s_sha3.
+        unfold safe_sstack_val_cmp_ext_1_d.
+        intros d' H_d'_le_0.
+        apply Nat.leb_le in H_d'_le_0 as H_d'_le_0_leb.
+        unfold safe_sstack_val_cmp.
+        intros.
+        destruct d'; try discriminate.
+        unfold sstack_val_cmp_fail_for_d_eq_0 in H_d0.
+        pose proof (H_d0 smemory_cmp sstorage_cmp sha3_cmp ctx sv1 sv2 maxidx1 sb1 maxidx2 sb2 ops).
+        rewrite H6 in H4.
+        discriminate.
+  - destruct IHd' as [IHd'_mem [IHd'_strg IHd'_sha3]].
+    pose proof (H_s_ssval d' smemory_cmp sstorage_cmp sha3_cmp IHd'_mem IHd'_strg IHd'_sha3) as H_s_ssval_Sd'.
+    apply safe_ext_2_implies_safe_ext_1 in H_s_ssval_Sd'.
+    split.
+    + apply H_s_mem.
+      apply H_s_ssval_Sd'.
+    + split.
+      * apply H_s_strg.
+        apply H_s_ssval_Sd'.
+      * apply H_s_sha3.
+        apply H_s_ssval_Sd'.
+Qed.
+
+
+Lemma safe_ext_sstack_val_cmp:
+  forall (smemory_cmp: smemory_cmp_ext_t) (sstorage_cmp: sstorage_cmp_ext_t) (sha3_cmp: sha3_cmp_ext_t) (sstack_val_cmp: sstack_val_cmp_ext_2_t),
+    sstack_val_cmp_fail_for_d_eq_0 sstack_val_cmp ->
+    safe_smemory_cmp_ext_wrt_sstack_value_cmp smemory_cmp ->
+    safe_sstorage_cmp_ext_wrt_sstack_value_cmp sstorage_cmp ->
+    safe_sha3_cmp_ext_wrt_sstack_value_cmp sha3_cmp ->
+    safe_sstack_value_cmp_wrt_others sstack_val_cmp ->
+    safe_sstack_val_cmp_ext_2 sstack_val_cmp smemory_cmp sstorage_cmp sha3_cmp.
+Proof.
+  intros smemory_cmp sstorage_cmp sha3_cmp sstack_val_cmp H_d0 H_s_mem H_s_strg H_s_sha3 H_s_ssval.
+  pose proof (safe_ext_smemory_sstorage_sha3_cmp smemory_cmp sstorage_cmp sha3_cmp sstack_val_cmp H_d0 H_s_mem H_s_strg H_s_sha3 H_s_ssval) as [H_smem [H_sstrg H_sha3]].
+  unfold safe_sstack_value_cmp_wrt_others in H_s_ssval.
+  unfold safe_sstack_val_cmp_ext_2.
+
+  destruct d as [|d'].
+  - unfold safe_sstack_val_cmp_ext_2_d.
+    unfold safe_sstack_val_cmp_ext_1_d.
+    intros d' H_d'_le_0.
+    apply Nat.leb_le in H_d'_le_0 as H_d'_le_0_leb.
+    unfold safe_sstack_val_cmp.
+    intros ctx sv1 sv2 maxidx1 sb1 maxidx2 sb2 ops H_is_sat H_valid_sv1 H_valid_sv2 H_valid_sb1 H_valid_sb2 H_sstack_val_cmp_fail_for_d_eq_0.
+    destruct d'; try discriminate.
+    unfold sstack_val_cmp_fail_for_d_eq_0 in H_d0.
+    pose proof (H_d0 smemory_cmp sstorage_cmp sha3_cmp ctx sv1 sv2 maxidx1 sb1 maxidx2 sb2 ops) as H_d0.
+    rewrite H_d0 in H_sstack_val_cmp_fail_for_d_eq_0.
+    discriminate.
+  -
+    unfold safe_smemory_cmp_ext in H_smem. pose proof (H_smem d') as H_smem.
+    unfold safe_sstorage_cmp_ext in H_sstrg. pose proof (H_sstrg d') as H_sstrg.
+    unfold safe_sha3_cmp_ext in H_sha3. pose proof (H_sha3 d') as H_sha3.
+    
+    pose proof (H_s_ssval d' smemory_cmp sstorage_cmp sha3_cmp H_smem H_sstrg H_sha3) as H_s_ssval_Sd'.
+
+    apply H_s_ssval_Sd'.
+Qed.
+
+
+Lemma safe_ext_all_cmp:
+  forall (smemory_cmp: smemory_cmp_ext_t) (sstorage_cmp: sstorage_cmp_ext_t) (sha3_cmp: sha3_cmp_ext_t) (sstack_val_cmp: sstack_val_cmp_ext_2_t),
+    sstack_val_cmp_fail_for_d_eq_0 sstack_val_cmp ->
+    safe_smemory_cmp_ext_wrt_sstack_value_cmp smemory_cmp ->
+    safe_sstorage_cmp_ext_wrt_sstack_value_cmp sstorage_cmp ->
+    safe_sha3_cmp_ext_wrt_sstack_value_cmp sha3_cmp ->
+    safe_sstack_value_cmp_wrt_others sstack_val_cmp ->
+    
+    safe_sstack_val_cmp_ext_2 sstack_val_cmp smemory_cmp sstorage_cmp sha3_cmp /\
+      safe_smemory_cmp_ext smemory_cmp (sstack_val_cmp smemory_cmp sstorage_cmp sha3_cmp) /\
+      safe_sstorage_cmp_ext sstorage_cmp (sstack_val_cmp smemory_cmp sstorage_cmp sha3_cmp) /\
+      safe_sha3_cmp_ext sha3_cmp (sstack_val_cmp smemory_cmp sstorage_cmp sha3_cmp).
+
+Proof.
+  intros smemory_cmp sstorage_cmp sha3_cmp sstack_val_cmp H_d0 H_s_mem H_s_strg H_s_sha3 H_s_ssval.
+  split.
+  - apply safe_ext_sstack_val_cmp.
+    + apply H_d0.
+    + apply H_s_mem.
+    + apply H_s_strg.
+    + apply H_s_sha3.
+    + apply H_s_ssval.
+  - apply safe_ext_smemory_sstorage_sha3_cmp.
+    + apply H_d0.
+    + apply H_s_mem.
+    + apply H_s_strg.
+    + apply H_s_sha3.
+    + apply H_s_ssval.
+Qed.
+
+Lemma safe_all_cmp:
+  forall (smemory_cmp: smemory_cmp_ext_t) (sstorage_cmp: sstorage_cmp_ext_t) (sha3_cmp: sha3_cmp_ext_t) (sstack_val_cmp: sstack_val_cmp_ext_2_t),
+    sstack_val_cmp_fail_for_d_eq_0 sstack_val_cmp ->
+    safe_smemory_cmp_ext_wrt_sstack_value_cmp smemory_cmp ->
+    safe_sstorage_cmp_ext_wrt_sstack_value_cmp sstorage_cmp ->
+    safe_sha3_cmp_ext_wrt_sstack_value_cmp sha3_cmp ->
+    safe_sstack_value_cmp_wrt_others sstack_val_cmp ->
+    forall d,
+    safe_sstack_val_cmp (sstack_val_cmp smemory_cmp sstorage_cmp sha3_cmp d) /\
+      safe_smemory_cmp (smemory_cmp (sstack_val_cmp smemory_cmp sstorage_cmp sha3_cmp d)) /\
+      safe_sstorage_cmp (sstorage_cmp (sstack_val_cmp smemory_cmp sstorage_cmp sha3_cmp d)) /\
+      safe_sha3_cmp (sha3_cmp (sstack_val_cmp smemory_cmp sstorage_cmp sha3_cmp d)).
+Proof.
+  intros smemory_cmp sstorage_cmp sha3_cmp sstack_val_cmp H_d0 H_s_mem H_s_strg H_s_sha3 H_s_ssval.
+  intro d.
+
+  pose proof (safe_ext_all_cmp smemory_cmp sstorage_cmp sha3_cmp sstack_val_cmp H_d0 H_s_mem H_s_strg H_s_sha3 H_s_ssval) as [H_safe_sstack_val_cmp_ext [H_safe_smemory_cmp_ext [H_safe_sstorage_cmp_ext H_safe_sha3_cmp_ext]]].
+
+  assert (H_d_le_d: d<=d). intuition.
+  repeat split.
+  - unfold safe_sstack_val_cmp_ext_2 in H_safe_sstack_val_cmp_ext.
+    unfold safe_sstack_val_cmp_ext_2_d in H_safe_sstack_val_cmp_ext.
+    unfold safe_sstack_val_cmp_ext_1_d in H_safe_sstack_val_cmp_ext.
+    apply H_safe_sstack_val_cmp_ext with (d:=d)(d':=d).
+    apply H_d_le_d.
+  - unfold safe_smemory_cmp_ext in H_safe_smemory_cmp_ext.
+    unfold safe_smemory_cmp_ext_d in H_safe_smemory_cmp_ext.    
+    apply H_safe_smemory_cmp_ext  with (d:=d)(d':=d).
+    apply H_d_le_d.
+  - unfold safe_sstorage_cmp_ext in H_safe_sstorage_cmp_ext.
+    unfold safe_sstorage_cmp_ext_d in H_safe_sstorage_cmp_ext.    
+    apply H_safe_sstorage_cmp_ext  with (d:=d)(d':=d).
+    apply H_d_le_d.
+  - unfold safe_sha3_cmp_ext in H_safe_sha3_cmp_ext.
+    unfold safe_sha3_cmp_ext_d in H_safe_sha3_cmp_ext.    
+    apply H_safe_sha3_cmp_ext  with (d:=d)(d':=d).
+    apply H_d_le_d.
+Qed.
+ 
+
+Lemma safe_smemory_cmp_ext_d_lt:
+  forall smemory_cmp sstack_val_cmp d1 d2,
+    d1 <= d2 ->
+    safe_smemory_cmp_ext_d smemory_cmp sstack_val_cmp d2 ->
+    safe_smemory_cmp_ext_d smemory_cmp sstack_val_cmp d1.
+Proof.
+  intros smemory_cmp sstack_val_cmp d1 d2 H_d1_le_d2 H_safe_smem_d2.
+  unfold safe_smemory_cmp_ext_d.
+  intros d' H_d'_lt_d1.
+  unfold safe_smemory_cmp_ext_d in H_safe_smem_d2.
+  apply H_safe_smem_d2.
+  intuition.
+Qed.
+
+Lemma safe_sstorage_cmp_ext_d_lt:
+  forall sstorage_cmp sstack_val_cmp d1 d2,
+    d1 <= d2 ->
+    safe_sstorage_cmp_ext_d sstorage_cmp sstack_val_cmp d2 ->
+    safe_sstorage_cmp_ext_d sstorage_cmp sstack_val_cmp d1.
+Proof.
+  intros sstorage_cmp sstack_val_cmp d1 d2 H_d1_le_d2 H_safe_sstrg_d2.
+  unfold safe_sstorage_cmp_ext_d.
+  intros d' H_d'_lt_d1.
+  unfold safe_sstorage_cmp_ext_d in H_safe_sstrg_d2.
+  apply H_safe_sstrg_d2.
+  intuition.
+Qed.
+
+Lemma safe_sha3_cmp_ext_d_lt:
+  forall sha3_cmp sstack_val_cmp d1 d2,
+    d1 <= d2 ->
+    safe_sha3_cmp_ext_d sha3_cmp sstack_val_cmp d2 ->
+    safe_sha3_cmp_ext_d sha3_cmp sstack_val_cmp d1.
+Proof.
+  intros sha3_cmp sstack_val_cmp d1 d2 H_d1_le_d2 H_safe_sha3_d2.
+  unfold safe_sha3_cmp_ext_d.
+  intros d' H_d'_lt_d1.
+  unfold safe_sha3_cmp_ext_d in H_safe_sha3_d2.
+  apply H_safe_sha3_d2.
+  intuition.
+Qed.
+
+Lemma safe_sstack_val_cmp_ext_2_d_le:
+  forall sstack_val_cmp smemory_cmp sstorage_cmp sha3_cmp d1 d2,
+    d1 <= d2 -> 
+    safe_sstack_val_cmp_ext_2_d sstack_val_cmp smemory_cmp sstorage_cmp sha3_cmp d2 ->
+    safe_sstack_val_cmp_ext_2_d sstack_val_cmp smemory_cmp sstorage_cmp sha3_cmp d1.
+Proof.
+Proof.
+  intros sstack_val_cmp smemory_cmp sstorage_cmp sha3_cmp d1 d2 H_d1_le_d2 H_safe_sstack_val_cmp_d2.
+  unfold safe_sstack_val_cmp_ext_2_d.
+  unfold safe_sstack_val_cmp_ext_1_d.
+  intros d' H_d'_lt_d1.
+  unfold safe_sstack_val_cmp_ext_2_d in H_safe_sstack_val_cmp_d2.
+  unfold safe_sstack_val_cmp_ext_1_d in H_safe_sstack_val_cmp_d2.
+  apply H_safe_sstack_val_cmp_d2.
+  intuition.
+Qed.
+
+
+End SymbolicStateCmp.
+
+  
